Add a version of typing where all the computations are stateTs only

src/Modify.v
@@ -26,16 +26,16 @@ Local Open Scope itree_scope.
 
 Ltac rewritebisim lem := pose proof lem as bisim;
                          eapply bisimulation_is_eq in bisim;
-                         rewrite bisim;
+                         setoid_rewrite bisim;
                          clear bisim.
 
 Ltac rewritebisim_in lem H := pose proof lem as bisim;
                               eapply bisimulation_is_eq in bisim;
-                              rewrite bisim in H;
+                              setoid_rewrite bisim in H;
                               clear bisim.
 
-Variant yieldE S : Type -> Type :=
-| Yield : S -> yieldE S S.
+Variant modifyE S : Type -> Type :=
+| Modify : (S -> S) -> modifyE S S.
 
 (** return one of the elements in [x :: xs], as well as the complete list of unchosen elements *)
 Fixpoint choose' {E} `{nondetE -< E} {X} (x : X) (xs : list X) (rest : list X) :
@@ -49,51 +49,51 @@ Fixpoint choose' {E} `{nondetE -< E} {X} (x : X) (xs : list X) (rest : list X) :
 Definition choose {E} `{nondetE -< E} {X} x xs : itree E (X * list X) :=
   choose' x xs [].
 
-Definition E config := yieldE config +' nondetE.
+Definition E config := modifyE config +' nondetE.
 
 Section parallel.
   Parameter config : Type.
 
   Definition thread := stateT config (itree (E config)) unit.
 
-  Definition par_match par (curr : thread) (rest : list thread)
-    : thread :=
-    fun s =>
-      match (observe (curr s)) with
+  Definition par_match par (curr : itree (E config) (config * unit)) (rest : list thread)
+    : itree (E config) (config * unit) :=
+    (* fun s => *)
+      match (observe curr) with
       | RetF (s', _) => match rest with
                        | [] => Ret (s', tt)
-                       | h :: t => Tau (par h t s')
+                       | h :: t => Tau (par (h s') t)
                        end
-      | TauF t => Tau (par (fun _ => t) rest s)
+      | TauF t => Tau (par t rest)
       | VisF (inl1 e) k =>
-        match e in yieldE _ C return (C -> itree (E config) (config * unit)) -> _ with
-        | Yield _ s' =>
+        match e in modifyE _ C return (C -> itree (E config) (config * unit)) -> _ with
+        | Modify _ f =>
           fun k' =>
           '(curr', rest') <- choose k' rest;;
-          Vis (inl1 (Yield _ s')) (fun s' => (par curr' rest' s'))
+          Vis (inl1 (Modify _ f)) (fun s' => (par (curr' s') rest'))
         end k
       | VisF (inr1 e) k =>
-        vis e (fun b => par (fun _ => k b) rest s)
+        vis e (fun b => par (k b) rest)
       end.
   CoFixpoint par := par_match par.
   Lemma rewrite_par curr rest : par curr rest = par_match par curr rest.
   Proof.
-    apply functional_extensionality. intros. apply bisimulation_is_eq.
-    revert x curr rest.
+    apply bisimulation_is_eq.
+    revert curr rest.
     ginit. gcofix CIH. intros. gstep. unfold par. red. reflexivity.
   Qed.
 
   Lemma par_single :
     forall t, par t [] = t.
   Proof.
-    intro. apply functional_extensionality. intros. apply bisimulation_is_eq.
-    revert t x. pcofix CIH. intros.
+    intros. apply bisimulation_is_eq.
+    revert t. pcofix CIH. intros.
     rewrite rewrite_par. unfold par_match.
-    destruct (observe (t x)) eqn:?; simpl; auto.
+    destruct (observe t) eqn:?; simpl; auto.
     - destruct r0. pstep. red. rewrite Heqi. simpl. destruct u. constructor; auto.
     - pstep. red. rewrite Heqi. constructor. right. apply CIH.
     - destruct e.
-      + destruct y. pstep. unfold choose. unfold choose'.
+      + destruct m. pstep. unfold choose. unfold choose'.
         rewritebisim @bind_ret_l.
   Abort.
 
@@ -118,29 +118,26 @@ Section parallel.
 End parallel.
 
 Variant typing_gen {R} typing (p : perm) (Q : config * R -> Perms) :
-  config -> itree (E config) (config * R) -> Prop :=
+  config -> stateT config (itree (E config)) R -> Prop :=
 | typing_gen_ret r c :
     pre p c ->
     (forall c', rely p c c' -> p ∈ Q (c', r)) ->
-    typing_gen typing p Q c (Ret (c, r))
-| typing_gen_tau t c p' :
-    pre p c ->
-    sep_step p p' -> (* Added since par turns vis into a tau, so the two cases need to be similar... *)
+    typing_gen typing p Q c (fun c => Ret (c, r))
+| typing_gen_tau t p' c :
+    sep_step p p' ->
     typing p' Q c t ->
-    typing_gen typing p Q c (Tau t)
-| typing_gen_vis k c c' p' :
+    typing_gen typing p Q c (fun c => Tau (t c))
+| typing_gen_vis k f p' c :
     pre p c ->
-    guar p c c' ->
-    (* pre p' c' -> *)
+    (forall c, pre p c -> guar p c (f c)) ->
     sep_step p p' ->
-    (forall c'', rely p c' c'' -> typing p' Q c'' (k c'')) ->
-    typing_gen typing p Q c (Vis (inl1 (Yield _ c')) k)
-(* other events. TODO: generalize E *)
+    (forall c', rely p (f c) c' -> typing p' Q c' (k)) ->
+    typing_gen typing p Q c (fun c => Vis (inl1 (Modify _ f)) k)
+(* (* other events. TODO: generalize E *) *)
 | typing_gen_e X c p' (e : nondetE X) k :
-    pre p c ->
     sep_step p p' ->
-    (forall x, typing p' Q c (k x)) ->
-    typing_gen typing p Q c (Vis (inr1 e) k)
+    (forall x, typing p' Q c (fun c => k x)) ->
+    typing_gen typing p Q c (fun c => Vis (inr1 e) k)
 .
 
 Lemma typing_gen_mon {R} : monotone4 (@typing_gen R).
@@ -151,7 +148,24 @@ Hint Resolve typing_gen_mon : paco.
 
 Definition typing_ {R} := paco4 (@typing_gen R) bot4.
 
-Lemma typing__lte {R} p Q Q' c (t : itree (E config) (config * R)) :
+Lemma typing__rely {R} p Q c c' (t : stateT config (itree (E config)) R) :
+  rely p c c' ->
+  typing_ p Q c t ->
+  typing_ p Q c' t.
+Proof.
+  revert p Q c c' t. pcofix CIH. intros p Q c c' t Hrely Ht.
+  pinversion Ht; subst.
+  - pstep. constructor. respects. intros. apply H0; auto. etransitivity; eauto.
+  - pstep. econstructor; eauto. right. eapply CIH; eauto. eapply sep_step_rely; eauto.
+  - pstep. econstructor; eauto. right. eapply CIH; eauto. eapply sep_step_rely; eauto.
+    assert (rely p (f c) (f c')) by admit.
+    assert (rely p (f c) c'0) by (etransitivity; eauto).
+    specialize (H2 _ H4). pclearbot. apply H2.
+  - pstep. econstructor; eauto. right. eapply CIH; eauto. eapply sep_step_rely; eauto.
+    apply H0.
+Admitted.
+
+Lemma typing__lte {R} p Q Q' c (t : stateT config (itree (E config)) R) :
   typing_ p Q c t ->
   (forall r, Q r ⊨ Q' r) ->
   typing_ p Q' c t.
@@ -160,7 +174,7 @@ Proof.
   pstep. pinversion Htyping; pclearbot; subst; econstructor; eauto.
   - intros. apply Hlte; eauto.
   - intros. specialize (H2 _ H3). pclearbot. eauto.
-  - intros. specialize (H1 x). eauto.
+  - intros. specialize (H0 x). eauto.
 Qed.
 
 (* Lemma typing__lte' p p' Q c (t : itree (E config) (config * unit)) : *)
@@ -175,11 +189,12 @@ Qed.
 (*     + eapply Perms_upwards_closed; eauto. *)
 (* Qed. *)
 
+(* Definition typing {R} P Q (t : stateT config (itree (E config)) R) := *)
+(*   forall p c, p ∈ P -> pre p c -> typing_ p Q (t c). *)
 Definition typing {R} P Q (t : stateT config (itree (E config)) R) :=
-  forall p c, p ∈ P -> pre p c -> typing_ p Q c (t c).
-(* also pre p c'? *)
+  forall p c, p ∈ P -> pre p c -> typing_ p Q c t.
 
-Lemma typing_lte {R} P P' Q Q' (t : stateT config (itree (E config)) R) :
+Lemma typing_lte {R} P P' (Q Q' : config * R -> Perms) t: (* (t : stateT config (itree (E config)) R) : *)
   typing P Q t ->
   P' ⊨ P ->
   (forall r, Q r ⊨ Q' r) ->
@@ -189,24 +204,36 @@ Proof.
 Qed.
 
 Lemma typing__bind {R S} p Q1 Q2 c
-      (t1 : itree (E config) (config * R))
+      (t1 : stateT config (itree (E config)) R)
       (t2 : R -> stateT config (itree (E config)) S)
       r' :
   typing_ p Q1 c t1 ->
   (forall r p c, (forall c', rely p c c' -> p ∈ Q1 (c', r)) ->
-             pre p c ->
-             paco4 typing_gen r' p Q2 c (t2 r c)) ->
-  paco4 typing_gen r' p Q2 c (x <- t1;; t2 (snd x) (fst x)).
+            pre p c ->
+            paco4 typing_gen r' p Q2 c (t2 r)) ->
+  paco4 typing_gen r' p Q2 c (fun c => x <- t1 c;; t2 (snd x) (fst x)).
 Proof.
   revert p Q1 Q2 c t1 t2. pcofix CIH. intros p Q1 Q2 c t1 t2 Ht1 Ht2.
   pinversion Ht1; subst.
-  - rewritebisim @bind_ret_l. eapply paco4_mon; eauto.
-  - rewritebisim @bind_tau. pstep. econstructor; eauto.
-  - rewritebisim @bind_vis. pstep. econstructor; eauto. intros.
+  - assert ((fun c0 => x <- Ret (c0, r0);; t2 (snd x) (fst x)) = (t2 r0)).
+    { apply functional_extensionality. intros. rewritebisim @bind_ret_l. auto. }
+    rewrite H1.
+    eapply paco4_mon; eauto.
+  - assert ((fun c0 : config => x <- Tau (t c0);; t2 (snd x) (fst x)) =
+            (fun c0 => Tau (x <- (t c0);; t2 (snd x) (fst x)))).
+    { apply functional_extensionality. intros. rewritebisim @bind_tau. auto. }
+    rewrite H1. pstep. econstructor; eauto.
+  - assert ((fun _ : config => x <- Vis (inl1 (Modify config f)) k;; t2 (snd x) (fst x)) =
+            (fun _ => Vis (inl1 (Modify config f)) (fun s => x <- k s;; t2 (snd x) (fst x)))).
+    { apply functional_extensionality. intros. rewritebisim @bind_vis. auto. }
+    rewrite H3. pstep. econstructor; eauto. intros.
     right. eapply CIH; eauto.
-    specialize (H2 _ H3). pclearbot. apply H2.
-  - rewritebisim @bind_vis. pstep. econstructor; eauto. intros.
-    right. eapply CIH; eauto. apply H1.
+    specialize (H2 _ H4). pclearbot. apply H2.
+  - assert ((fun _ : config => x <- Vis (inr1 e) k;; t2 (snd x) (fst x)) =
+            (fun _ => Vis (inr1 e) (fun x => x <- k x;; t2 (snd x) (fst x)))).
+    { apply functional_extensionality. intros. rewritebisim @bind_vis. auto. }
+    rewrite H1. pstep. econstructor; eauto. intros.
+    right. eapply CIH; eauto. apply H0.
 Qed.
 
 Lemma typing_bind {R S} P Q1 Q2
@@ -216,157 +243,170 @@ Lemma typing_bind {R S} P Q1 Q2
   (forall c r, typing (Q1 (c, r)) Q2 (t2 r)) ->
   typing P Q2 (bind t1 t2).
 Proof.
-  repeat intro. unfold bind. unfold Monad_stateT. red.
-  eapply typing__bind; eauto. intros. eapply H0; eauto. apply H3; auto. reflexivity.
+  intros Ht1 Ht2 p c Hp Hpre.
+  eapply typing__bind; eauto. intros. eapply Ht2; eauto. apply H; reflexivity.
 Qed.
 
-Lemma typing__tau p (Q : config * unit -> Perms) c t :
+Lemma typing__tau {R} p (Q : config * R -> Perms) c t :
   typing_ p Q c t ->
-  typing_ p Q c (Tau t).
+  typing_ p Q c (fun c => Tau (t c)).
 Proof.
   intros Ht.
-  pinversion Ht; subst; simpl.
-  - pstep. econstructor; eauto. reflexivity.
-  - pstep. econstructor; auto. reflexivity. left. pstep. econstructor; eauto.
-  - pstep. econstructor; auto. reflexivity. left. pstep. econstructor; eauto.
-  - pstep. econstructor; auto. reflexivity. left. pstep. econstructor; eauto.
+  pinversion Ht; subst; simpl; try solve [pstep; econstructor; try reflexivity; eauto].
 Qed.
 
-
-Lemma typing__par_empty p Q c c' t :
-  typing_ p Q c (t c') ->
-  typing_ p Q c (par t [] c').
+(* TODO after this point *)
+Lemma typing__par_empty p Q c t :
+  typing_ p Q c t ->
+  typing_ p Q c (par t []).
 Proof.
-  revert p c c' t.
+  revert p t.
   pcofix CIH.
-  intros p c c' t Ht. rewrite rewrite_par. unfold par_match.
+  intros p t Ht. rewrite rewrite_par. unfold par_match.
   pinversion Ht; subst; simpl.
-  - pstep. constructor; auto. destruct r0; auto.
+  - destruct r0. pstep. constructor; auto.
   - pstep. econstructor; eauto.
-  - pstep. unfold choose, choose'. rewritebisim @bind_ret_l. econstructor; eauto.
+  - pstep. unfold choose, choose'. rewritebisim @bind_ret_l.
+    econstructor; eauto.
+    clear Ht H.
     right. eapply CIH; eauto.
-    assert (rely p c'0 c'0) by reflexivity.
-    specialize (H4 _ H3). pclearbot.
-    apply H4.
-  - pstep. econstructor; eauto. intros. right. apply CIH. apply H3.
+    specialize (H1 _ _ H H2). pclearbot. eauto.
+  - pstep. econstructor; eauto. intros. right. apply CIH. apply H0.
 Qed.
 
 Lemma typing_par_empty P Q t :
   typing P Q t ->
   typing P Q (par t []).
 Proof.
-  intros Ht p c Hp Hpre. apply typing__par_empty; auto.
+  intros Ht p Hp. apply typing__par_empty; auto.
 Qed.
 
 Lemma typing__frame p p' r (Q : config * unit -> Perms) R t c :
-  typing_ p Q c t ->
+  typing_ p Q (t c) ->
   r ∈ R ->
   p ** r <= p' ->
   pre p' c ->
-  typing_ p' (fun c => Q c * R) c t.
+  typing_ p' (fun c' => Q c' * R) (t c).
 Proof.
-  revert p p' r Q R t c.
-  pcofix CIH. intros p p' r' Q R t c Ht Hr Hp' Hpre.
-  pinversion Ht; subst.
-  - pstep. constructor; auto. destruct r0. intros.
-    eapply Perms_upwards_closed; eauto. apply sep_conj_Perms_perm; auto.
-    apply H0; auto. apply Hp'; auto.
-  - pstep. econstructor; auto.
-    + eapply sep_step_lte; eauto. eapply sep_step_sep_conj_l.
-      apply Hp' in Hpre. apply Hpre.
-      apply H0.
-    + right. eapply CIH; eauto. reflexivity.
-      split; [| split]. pinversion H1; auto.
-      apply Hp'. apply Hpre.
-      apply H0. apply Hp' in Hpre. apply Hpre.
-  - pstep. econstructor; auto.
-    + apply Hp'. constructor. left. auto.
-    + eapply sep_step_lte; eauto. eapply sep_step_sep_conj_l.
-      apply Hp' in Hpre. apply Hpre.
-      apply H1.
-    + intros. right.
-      assert (rely p c' c'').
-      { apply Hp'. auto. }
-      specialize (H2 _ H4). pclearbot.
-      eapply CIH; eauto. reflexivity.
-      split; [| split].
-      * pinversion H2; auto.
-      * pose proof Hpre as Hpre'. apply Hp' in Hpre'. destruct Hpre' as (_ & _ & Hsep).
-        apply Hsep in H0. respects. etransitivity; eauto. apply Hp'. auto. apply Hp'; auto.
-      * apply H1. apply Hp' in Hpre. apply Hpre.
-  - pstep. econstructor; eauto.
-    + eapply sep_step_lte; eauto. eapply sep_step_sep_conj_l.
-      apply Hp' in Hpre. apply Hpre.
-      apply H0.
-    + intros. specialize (H1 x). right. eapply CIH; eauto. reflexivity.
-      split; [| split]. pinversion H1; auto.
-      apply Hp'. auto.
-      apply Hp' in Hpre. apply H0. apply Hpre.
-Qed.
+(*   revert p p' r Q R t c. *)
+(*   pcofix CIH. intros p p' r' Q R t c Ht Hr Hp' Hpre. *)
+(*   pinversion Ht; subst. *)
+(*   - destruct r0. pstep. constructor; auto. *)
+(*     apply Hp'. *)
+(*     eapply Perms_upwards_closed; eauto. apply sep_conj_Perms_perm; auto. *)
+(*     apply H0; auto. apply Hp'; auto. *)
+(*   - pstep. econstructor; auto. *)
+(*     + eapply sep_step_lte; eauto. eapply sep_step_sep_conj_l. *)
+(*       apply Hp' in Hpre. apply Hpre. *)
+(*       apply H0. *)
+(*     + right. eapply CIH; eauto. reflexivity. *)
+(*       split; [| split]. pinversion H1; auto. *)
+(*       apply Hp'. apply Hpre. *)
+(*       apply H0. apply Hp' in Hpre. apply Hpre. *)
+(*   - pstep. econstructor; auto. *)
+(*     + apply Hp'. constructor. left. auto. *)
+(*     + eapply sep_step_lte; eauto. eapply sep_step_sep_conj_l. *)
+(*       apply Hp' in Hpre. apply Hpre. *)
+(*       apply H1. *)
+(*     + intros. right. *)
+(*       assert (rely p c' c''). *)
+(*       { apply Hp'. auto. } *)
+(*       specialize (H2 _ H4). pclearbot. *)
+(*       eapply CIH; eauto. reflexivity. *)
+(*       split; [| split]. *)
+(*       * pinversion H2; auto. *)
+(*       * pose proof Hpre as Hpre'. apply Hp' in Hpre'. destruct Hpre' as (_ & _ & Hsep). *)
+(*         apply Hsep in H0. respects. etransitivity; eauto. apply Hp'. auto. apply Hp'; auto. *)
+(*       * apply H1. apply Hp' in Hpre. apply Hpre. *)
+(*   - pstep. econstructor; eauto. *)
+(*     + eapply sep_step_lte; eauto. eapply sep_step_sep_conj_l. *)
+(*       apply Hp' in Hpre. apply Hpre. *)
+(*       apply H0. *)
+(*     + intros. specialize (H1 x). right. eapply CIH; eauto. reflexivity. *)
+(*       split; [| split]. pinversion H1; auto. *)
+(*       apply Hp'. auto. *)
+(*       apply Hp' in Hpre. apply H0. apply Hpre. *)
+(* Qed. *)
+Abort.
 
-Lemma typing__frame' p p' r (Q R : config * unit -> Perms) t c :
-  typing_ p Q c t ->
-  (forall c', rely r c c' -> r ∈ R (c', tt)) ->
-  r ** p <= p' ->
-  pre p' c ->
-  typing_ p' (fun c => R c * Q c) c t.
-Proof.
-  revert p p' r Q R t c.
-  pcofix CIH. intros p p' r' Q R t c Ht Hr Hp' Hpre.
-  pinversion Ht; subst.
-  - pstep. constructor; auto. destruct r0. intros.
-    eapply Perms_upwards_closed; eauto. apply sep_conj_Perms_perm; auto.
-    + apply Hr; auto. apply Hp'; auto.
-    + apply H0; auto. apply Hp'; auto.
-  - pstep. econstructor; auto.
-    + eapply sep_step_lte; eauto. eapply sep_step_sep_conj_r.
-      apply Hp' in Hpre. destruct Hpre as (_ & _ & Hpre). symmetry in Hpre. apply Hpre.
-      apply H0.
-    + right. eapply CIH; eauto. reflexivity.
-      (* intros. apply Hr. apply Hp'. eapply sep_step_rely; eauto. *)
+(* Lemma typing__frame' p p' r (Q R : config * unit -> Perms) t c : *)
+(*   typing_ p Q c t -> *)
+(*   (forall c', rely r c c' -> r ∈ R (c', tt)) -> *)
+(*   r ** p <= p' -> *)
+(*   pre p' c -> *)
+(*   typing_ p' (fun c => R c * Q c) c t. *)
+(* Proof. *)
+(*   revert p p' r Q R t c. *)
+(*   pcofix CIH. intros p p' r' Q R t c Ht Hr Hp' Hpre. *)
+(*   pinversion Ht; subst. *)
+(*   - pstep. constructor; auto. destruct r0. intros. *)
+(*     eapply Perms_upwards_closed; eauto. apply sep_conj_Perms_perm; auto. *)
+(*     + apply Hr; auto. apply Hp'; auto. *)
+(*     + apply H0; auto. apply Hp'; auto. *)
+(*   - pstep. econstructor; auto. *)
+(*     + eapply sep_step_lte; eauto. eapply sep_step_sep_conj_r. *)
+(*       apply Hp' in Hpre. destruct Hpre as (_ & _ & Hpre). symmetry in Hpre. apply Hpre. *)
+(*       apply H0. *)
+(*     + right. eapply CIH; eauto. reflexivity. *)
+(*       (* intros. apply Hr. apply Hp'. eapply sep_step_rely; eauto. *) *)
 
-      split; [| split].
-      apply Hp'. apply Hpre.
-      pinversion H1; auto.
-      symmetry. apply H0. apply Hp' in Hpre.
-      destruct Hpre as (_ & _ & Hpre). symmetry in Hpre. apply Hpre.
-  - pstep. econstructor; eauto.
-    + apply Hp'. constructor. right. auto.
-    + eapply sep_step_lte; eauto. eapply sep_step_sep_conj_r; eauto.
-      apply Hp' in Hpre. destruct Hpre as (_ & _ & Hpre). symmetry in Hpre. apply Hpre.
-    + intros. right.
-      assert (rely p c' c'').
-      { apply Hp'. auto. }
-      specialize (H2 _ H4). pclearbot.
-      eapply CIH; eauto. 2: reflexivity.
+(*       split; [| split]. *)
+(*       apply Hp'. apply Hpre. *)
+(*       pinversion H1; auto. *)
+(*       symmetry. apply H0. apply Hp' in Hpre. *)
+(*       destruct Hpre as (_ & _ & Hpre). symmetry in Hpre. apply Hpre. *)
+(*   - pstep. econstructor; eauto. *)
+(*     + apply Hp'. constructor. right. auto. *)
+(*     + eapply sep_step_lte; eauto. eapply sep_step_sep_conj_r; eauto. *)
+(*       apply Hp' in Hpre. destruct Hpre as (_ & _ & Hpre). symmetry in Hpre. apply Hpre. *)
+(*     + intros. right. *)
+(*       assert (rely p c' c''). *)
+(*       { apply Hp'. auto. } *)
+(*       specialize (H2 _ H4). pclearbot. *)
+(*       eapply CIH; eauto. 2: reflexivity. *)
 
-      intros. apply Hr. etransitivity; eauto.
-      apply Hp' in Hpre. destruct Hpre as (_ & _ & Hsep). transitivity c'.
-      apply Hsep; auto. apply Hp'; auto.
+(*       intros. apply Hr. etransitivity; eauto. *)
+(*       apply Hp' in Hpre. destruct Hpre as (_ & _ & Hsep). transitivity c'. *)
+(*       apply Hsep; auto. apply Hp'; auto. *)
 
-      split; [| split].
-      * pose proof Hpre as Hpre'. apply Hp' in Hpre'. destruct Hpre' as (_ & _ & Hsep).
-        apply Hsep in H0. respects. etransitivity; eauto. apply Hp'. auto. apply Hp'; auto.
-      * pinversion H2; auto.
-      * symmetry. apply H1. apply Hp' in Hpre.
-        destruct Hpre as (_ & _ & Hpre). symmetry in Hpre. apply Hpre.
-  - pstep. econstructor; eauto.
-    + eapply sep_step_lte; eauto. eapply sep_step_sep_conj_r; eauto.
-      apply Hp' in Hpre. destruct Hpre as (_ & _ & Hpre). symmetry in Hpre. apply Hpre.
-    + intros. specialize (H1 x). right. eapply CIH; eauto. reflexivity.
-      split; [| split].
-      apply Hp'. auto.
-      pinversion H1; auto.
-      symmetry. apply Hp' in Hpre. apply H0.
-      destruct Hpre as (_ & _ & Hpre). symmetry in Hpre. apply Hpre.
-Qed.
+(*       split; [| split]. *)
+(*       * pose proof Hpre as Hpre'. apply Hp' in Hpre'. destruct Hpre' as (_ & _ & Hsep). *)
+(*         apply Hsep in H0. respects. etransitivity; eauto. apply Hp'. auto. apply Hp'; auto. *)
+(*       * pinversion H2; auto. *)
+(*       * symmetry. apply H1. apply Hp' in Hpre. *)
+(*         destruct Hpre as (_ & _ & Hpre). symmetry in Hpre. apply Hpre. *)
+(*   - pstep. econstructor; eauto. *)
+(*     + eapply sep_step_lte; eauto. eapply sep_step_sep_conj_r; eauto. *)
+(*       apply Hp' in Hpre. destruct Hpre as (_ & _ & Hpre). symmetry in Hpre. apply Hpre. *)
+(*     + intros. specialize (H1 x). right. eapply CIH; eauto. reflexivity. *)
+(*       split; [| split]. *)
+(*       apply Hp'. auto. *)
+(*       pinversion H1; auto. *)
+(*       symmetry. apply Hp' in Hpre. apply H0. *)
+(*       destruct Hpre as (_ & _ & Hpre). symmetry in Hpre. apply Hpre. *)
+(* Qed. *)
 
 Lemma typing_frame P P' (Q : config * unit -> Perms) t :
   typing P Q t ->
   typing (P * P') (fun r => Q r * P') t.
 Proof.
-  repeat intro. destruct H0 as (? & ? & ? & ? & ?).
-  eapply typing__frame; eauto. apply H; auto. apply H3. auto.
+  intros Ht p'' (p & p' & Hp & Hp' & Hlte).
+  specialize (Ht _ Hp).
+  revert Ht Hp Hp' Hlte. revert P P' Q t p p'' p'.
+  pcofix CIH. intros. pinversion Ht; subst; simpl.
+  - destruct r0. pstep. constructor; auto.
+    admit.
+    intros. eapply Perms_upwards_closed; eauto.
+    apply sep_conj_Perms_perm; auto. apply H0. apply Hlte; auto.
+  - pstep. econstructor; auto.
+    + eapply sep_step_lte; eauto. eapply sep_step_sep_conj_l.
+      apply Hp' in Hpre. apply Hpre.
+      apply H0.
+
+    2: {
+      right. eapply CIH; eauto.
+
+    eapply typing__frame; eauto. apply H; auto. apply H3. auto.
 Qed.
 
 Lemma typing_rely p (Q : config * unit -> Perms) t c c' :
